Package passing of interpreter values (#2)
* adding an incremental Makefile; dune files for the OCaml build; and an .fst.config.json file for use with fstar-vscode-assistant

* name

* use an iresult monad to factor out passing interpreter state by value

---------

Co-authored-by: Anand Krishnamoorthi <35780660+anakrish@users.noreply.github.com>

Rego.Interpreter.fst
@@ -13,9 +13,16 @@ let make_new () = {
    scopes = [];
    loop_exprs = [];
 }
+let iresult a = intr -> a & intr
+let (let!) #a #b (f:iresult a) (g:a -> iresult b) : iresult b = fun i -> let (a', i') = f i in g a' i'
+let return #a (x:a) : iresult a = fun i -> (x, i)
+let get () : iresult intr = fun i -> (i, i)
+let set i : iresult unit = fun _ -> ((), i)
+let run #a (f:iresult a) (i:intr) : a & intr = f i
 
-let lookup_loop_var (i:intr) (e:expr) =
-    List.Tot.find (fun (k,_) -> k = e) i.loop_exprs
+let lookup_loop_var (e:expr) : iresult _ = 
+  let! i = get() in
+  return <| List.Tot.find (fun (k,_) -> k = e) i.loop_exprs
 
 let rec lookup_var_in_scopes (scopes:list scope) (name:string) =
     match scopes with
@@ -25,123 +32,141 @@ let rec lookup_var_in_scopes (scopes:list scope) (name:string) =
       | None -> lookup_var_in_scopes tl name)
     | _ -> Undefined
 
-let lookup_local_var (i:intr) (name:string) =
-    lookup_var_in_scopes i.scopes name
+let lookup_local_var (name:string) : iresult value =
+    let! i = get () in
+    return <| lookup_var_in_scopes i.scopes name
 
-let rec eval_expr (e:expr) (i:intr)  : Tot (value*intr)
-=
-  match lookup_loop_var i e with
-  | Some((_, v)) -> (v, i)
+
+let lookup_var (ident:string)
+: iresult value
+= lookup_local_var ident
+
+let rec eval_expr (e:expr)
+: iresult value
+= match! lookup_loop_var e with
+  | Some((_, v)) -> return v
   | None ->
-  match e with
-  | Var v -> lookup_var v i
-  | Value v -> (v, i)
-  | Ast.Array elems -> eval_array_elems elems [] i
-  | Ast.Set elems -> eval_set_elems elems [] i
-  | Ast.Object fields -> eval_fields fields (Object []) i
-  | Ast.ArrayCompr query -> eval_query_stmts query.stmts (Value.Array []) i
-  | Ast.SetCompr query -> eval_query_stmts query.stmts (Value.Set []) i
-  | Ast.ObjectCompr query -> eval_query_stmts query.stmts (Value.Object []) i
-  | Ast.RefDot (refr, field) -> eval_ref_dot refr (field, i)
-  | Ast.RefBrack (refr, index) -> eval_ref_brack (refr, index) i
-  | Ast.AssignExpr (op, lhs, rhs) -> eval_assign_expr (op, lhs, rhs) i
-  | _ -> (Undefined, i)
+    match e with
+    | Var v -> lookup_var v
+    | Value v -> return v
+    | Ast.Array elems -> eval_array_elems elems []
+    | Ast.Set elems -> eval_set_elems elems [] 
+    | Ast.Object fields -> eval_fields fields (Object [])
+    | Ast.ArrayCompr query -> eval_query_stmts query.stmts (Value.Array [])
+    | Ast.SetCompr query -> eval_query_stmts query.stmts (Value.Set [])
+    | Ast.ObjectCompr query -> eval_query_stmts query.stmts (Value.Object [])
+    | Ast.RefDot rf -> eval_ref_dot rf
+    | Ast.RefBrack ri -> eval_ref_brack ri
+    | Ast.AssignExpr olr -> eval_assign_expr olr
+    | _ -> return Undefined
 
-
-and eval_array_elems (elems:list expr) (values:list value) (i:intr)  : Tot (value*intr)
-=
-  match elems with
-  | [] -> (Value.Array (List.Tot.rev values), i)
+and eval_array_elems (elems:list expr) (values:list value)
+: iresult value
+= match elems with
+  | [] -> return <| Value.Array (List.Tot.rev values)
   | hd::tl ->
-    match eval_expr hd i with
-    | (Undefined, i') -> (Undefined, i')
-    | (v, i') -> eval_array_elems tl (v::values) i'
+    match! eval_expr hd with
+    | Undefined -> return Undefined
+    | v -> eval_array_elems tl (v::values)
 
-and eval_set_elems (elems:list expr) (values:list value) (i:intr)  : Tot (value*intr)
-=
-  match elems with
-  | [] -> (List.Tot.fold_left Value.insert_into_set (Value.Set []) values, i)
+and eval_set_elems (elems:list expr) (values:list value)
+: iresult value
+= match elems with
+  | [] -> return <| List.Tot.fold_left Value.insert_into_set (Value.Set []) values
   | hd::tl ->
-    match eval_expr hd i with
-    | (Undefined, i') -> (Undefined, i')
-    | (v, i') -> eval_set_elems tl (v::values) i'
+    match! eval_expr hd with
+    | Undefined -> return Undefined
+    | v -> eval_set_elems tl (v::values)
 
-and eval_fields (fields:list (expr*expr)) (obj:value) (i:intr)  : Tot (value*intr)
-=
-  match fields with
-  | [] -> (obj, i)
+and eval_fields (fields:list (expr*expr)) (obj:value)
+: iresult value
+= match fields with
+  | [] -> return obj
   | (key_expr,value_expr)::tl ->
-    match eval_expr key_expr i with
-    | (Undefined, i') -> (Undefined, i')
-    | (kv, i') ->
-      match eval_expr value_expr i' with
-      | (Undefined, i'') -> (Undefined, i'')
-      | (vv, i'') -> eval_fields tl (insert_into_object obj kv vv) i''
+    match! eval_expr key_expr with
+    | Undefined -> return Undefined
+    | kv ->
+      match! eval_expr value_expr with
+      | Undefined -> return Undefined
+      | vv -> eval_fields tl (insert_into_object obj kv vv)
 
-and lookup_var (ident:string) (i:intr)  : Tot (value*intr)
-=
-  (lookup_local_var i ident, i)
 
-and eval_query_stmts (stmts:list literalStmt) (out:value) (i:intr) : Tot (value*intr)
-=
-  match stmts with
-  | hd::[] ->
-    (match hd.literal with
+and eval_query_stmts (stmts:list literalStmt) (out:value)
+: iresult value
+= match stmts with
+  | [] -> return Undefined
+  
+  | [hd] -> (
+    match hd.literal with
     | ArrayComprOutput e ->
-      let (v, i') = eval_expr e i in
-      (insert_into_array out v, i')
+      let! v = eval_expr e in
+      return <| insert_into_array out v
     | SetComprOutput e ->
-      let (v, i') = eval_expr e i in
-      (insert_into_set out v, i')
+      let! v = eval_expr e in
+      return <| insert_into_set out v
     | ObjectComprOutput (ke, ve) ->
-      let (kv, i') = eval_expr ke i in
-      let (vv, i'') = eval_expr ve i' in
-      (insert_into_object out kv vv, i')
-    | _ -> (Undefined, i))
+      let! kv = eval_expr ke in
+      let! vv = eval_expr ve in
+      return <| insert_into_object out kv vv
+    | _ -> 
+      return Undefined
+  )
+
   | hd::tl ->
-    let (v, i') = match hd.literal with
-    | Expr e -> eval_expr e i
-    | _ -> (Undefined, i)
-    in eval_query_stmts tl out i'
-  | [] -> (Undefined, i)
+    (* we evaluate hd and just ignore the result, we only care about the side effects? *)
+    let! _v = 
+      match hd.literal with
+      | Expr e -> eval_expr e
+      | _ -> return Undefined
+    in
+    eval_query_stmts tl out
+
+  
+(* todo chaining *)
+and eval_ref_dot rf
+: iresult value
+= let refr, field = rf in
+  let! v = eval_expr refr in
+  return <| lookup_path v [Value.String field]
 
 (* todo chaining *)
-and eval_ref_dot (refr:expr) pr  : Tot (value*intr)
-=
-    let (field, i) = pr in
-    let (v, i') = eval_expr refr i in
-    (lookup_path v (Value.String field::[]), i')
-
-(* todo chaining *)
-and eval_ref_brack (pr:expr*expr) (i:intr)  : Tot (value*intr)
-=
-    let (refr, index) = pr in
-    let (v, i') = eval_expr refr i in
-    let (idx, i'') = eval_expr index i' in
-    (lookup_path v (idx::[]), i'')
+and eval_ref_brack (pr:expr*expr)
+: Tot (iresult value) (decreases pr)
+= let refr, index = pr in
+  let! v = eval_expr refr in
+  let! idx = eval_expr index in
+  return <| lookup_path v (idx::[])
 
 (* todo...actual implementation is quite complex *)
-and eval_assign_expr (t: (assignOp*expr*expr)) (i:intr) : Tot (value*intr)
-=
-  let (_, lhs, rhs) = t in
+and eval_assign_expr (t: (assignOp*expr*expr))
+: iresult value
+= let (_, lhs, rhs) = t in
   match lhs with
-  | Var name ->
-    (
-      let (rv, i') = eval_expr rhs i in
-      match rv with
-      | Undefined -> (Undefined, i')
-      | _ -> (* todo check existing binding *)
-        match i'.scopes with
-        | hd::tl -> (Bool true, {i' with scopes = ((name, rv)::hd)::tl})
-        | _ -> (Undefined, i')
+  | Var name -> (
+    let! rv = eval_expr rhs in
+    match rv with
+    | Undefined ->
+      return Undefined
+    | _ -> (* todo check existing binding *)
+      let! i = get() in
+      match i.scopes with
+      | hd::tl -> 
+        set {i with scopes = ((name, rv)::hd)::tl};!
+        return <| Bool true
+      | _ -> 
+        return Undefined
     )
-  | _ -> (Undefined, i)
-
-
+  | _ ->
+    return Undefined
 
 let eval (i:intr) (e:Ast.expr) : (value*intr) =
-  eval_expr e i
+  run (eval_expr e) i
+
+let eval_user_query' (q:Ast.query)
+: iresult value
+= let! i = get() in
+  set { i with scopes = []::i.scopes } ;!
+  eval_query_stmts q.stmts (Value.Array [])
 
 let eval_user_query (i:intr) (q:Ast.query) : (value*intr) =
-  let i' = { i with scopes = []::i.scopes } in
-  eval_query_stmts q.stmts (Value.Array []) i'
+  run (eval_user_query' q) i
